\input{../utils/preamble}
\createdgmtitle{12}

\usepackage{tikz}

\usetikzlibrary{arrows,shapes,positioning,shadows,trees}
%--------------------------------------------------------------------------------
\begin{document}
%--------------------------------------------------------------------------------
\begin{frame}[noframenumbering,plain]
%\thispagestyle{empty}
\titlepage
\end{frame}
%=======
\begin{frame}{Recap of previous lecture}
	\begin{block}{Theorem (Kolmogorov-Fokker-Planck: special case)}
		If $\bff$ is uniformly Lipschitz continuous in $\bz$ and continuous in $t$, then
		\[
			\frac{d \log p(\bz(t), t)}{d t} = - \text{tr} \left( \frac{\partial \bff_{\btheta}(\bz(t), t)}{\partial \bz(t)} \right).
		\]
		\[
			\log p(\bz(t_1), t_1) = \log p(\bz(t_0), t_0) - \int_{t_0}^{t_1} \text{tr}  \left( \frac{\partial \bff_{\btheta}(\bz(t), t)}{\partial \bz(t)} \right) dt.
		\]
	\end{block}
	\vspace{-0.3cm}
	\begin{itemize}
		\item \textbf{Discrete-in-time NF}: evaluation of determinant of the Jacobian costs $O(m^3)$ (we need invertible $\bff$).
		\item \textbf{Continuous-in-time NF}: getting the trace of the Jacobian costs $O(m^2)$ (we need smooth $\bff$).
	\end{itemize}
	\begin{block}{Hutchinson's trace estimator}
		\vspace{-0.3cm}
		\[
  \log p(\bz(t_1)) = \log p(\bz(t_0)) - \mathbb{E}_{p(\bepsilon)} \int_{t_0}^{t_1} \left[ {\color{violet}\bepsilon^T \frac{\partial \bff}{\partial \bz}} \bepsilon \right] dt.
		\]
	\end{block}
	\myfootnotewithlink{https://arxiv.org/abs/1810.01367}{Grathwohl W. et al. FFJORD: Free-form Continuous Dynamics for Scalable Reversible Generative Models, 2018} 
\end{frame}
%=======
\begin{frame}{Recap of previous lecture}
	\begin{block}{Forward pass (Loss function)}
		\vspace{-0.3cm}
		\[
			\bz = \bx + \int_{t_1}^{t_0} \bff_{\btheta}(\bz(t), t) dt, \quad L(\bz) = - \log p(\bx | \btheta)
		\]
		\[
			L(\bz) = - \log p(\bz) + \int_{t_0}^{t_1} \text{tr} \left( \frac{\partial \bff_{\btheta}(\bz(t), t)}{\partial \bz(t)} \right) dt
		\]
		\vspace{-0.5cm}
	\end{block}
	\begin{block}{Adjoint functions}
		\vspace{-0.4cm}
		\[
			\ba_{\bz}(t) = \frac{\partial L}{\partial \bz(t)}; \quad \ba_{\btheta}(t) = \frac{\partial L}{\partial \btheta(t)}.
		\]
		These functions show how the gradient of the loss depends on the hidden state~$\bz(t)$ and parameters $\btheta$.
		\vspace{-0.3cm}
	\end{block}

	\begin{block}{Theorem (Pontryagin)}
		\vspace{-0.6cm}
		\[
		\frac{d \ba_{\bz}(t)}{dt} = - \ba_{\bz}(t)^T \cdot \frac{\partial \bff_{\btheta}(\bz(t), t)}{\partial \bz}; \quad \frac{d \ba_{\btheta}(t)}{dt} = - \ba_{\bz}(t)^T \cdot \frac{\partial \bff_{\btheta}(\bz(t),  t)}{\partial \btheta}.
		\]
		\vspace{-0.7cm}
	\end{block}

	\myfootnotewithlink{https://arxiv.org/abs/1806.07366}{Chen R. T. Q. et al. Neural Ordinary Differential Equations, 2018}     
\end{frame}
%=======
\begin{frame}{Recap of previous lecture}
	\begin{block}{Forward pass}
		\vspace{-0.3cm}
		\[
		\bz = \bz(t_0) = \int^{t_1}_{t_0} \bff_{\btheta}(\bz(t), t) d t  + \bx \quad \Rightarrow \quad \text{ODE Solver}
		\]
		\vspace{-0.4cm}
	\end{block}
	\begin{block}{Backward pass}
		\vspace{-0.5cm}
		\begin{equation*}
			\left.
			{\footnotesize 
				\begin{aligned}
					\frac{\partial L}{\partial \btheta(t_1)} &= \ba_{\btheta}(t_1) =  - \int_{t_0}^{t_1} \ba_{\bz}(t)^T \frac{\partial \bff_{\btheta}(\bz(t), t)}{\partial \btheta(t)} dt + 0 \\
					\frac{\partial L}{\partial \bz(t_1)} &= \ba_{\bz}(t_1) =  - \int_{t_0}^{t_1} \ba_{\bz}(t)^T \frac{\partial \bff_{\btheta}(\bz(t), t)}{\partial \bz(t)} dt + \frac{\partial L}{\partial \bz(t_0)} \\
					\bz(t_1) &= - \int^{t_0}_{t_1} \bff_{\btheta}(\bz(t), t) d t  + \bz_0.
				\end{aligned}
			}
			\right\rbrace
			\Rightarrow
			\text{ODE Solver}
		\end{equation*}
		\vspace{-0.4cm} 
	\end{block}
	\textbf{Note:} These scary formulas are the standard backprop in the discrete case.
	\myfootnotewithlink{https://arxiv.org/abs/1806.07366}{Chen R. T. Q. et al. Neural Ordinary Differential Equations, 2018}   
\end{frame}
%=======
\begin{frame}{Recap of previous lecture}
	\vspace{-0.2cm}
	\begin{block}{SDE basics}
		Let define stochastic process $\bx(t)$ with initial condition $\bx(0) \sim p_0(\bx)$:
		\[
			d\bx = \mathbf{f}(\bx, t) dt + g(t) d \bw, 
		\]
		where $\bw(t)$ is the standard Wiener process (Brownian motion)
		\vspace{-0.2cm}
		\[		
			\bw(t) - \bw(s) \sim \cN(0, (t - s) \bI), \quad d \bw = \bepsilon \cdot \sqrt{dt}, \, \text{where } \bepsilon \sim \cN(0, \bI).
		\]
	\end{block}
	\vspace{-0.5cm}
	\begin{block}{Langevin dynamics}
		Let $\bx_0$ be a random vector. Then under mild regularity conditions for small enough $\eta$ samples from the following dynamics
		\vspace{-0.2cm}
		\[
			\bx_{t + 1} = \bx_t + \eta \frac{1}{2} \nabla_{\bx_t} \log p(\bx_t | \btheta) + \sqrt{\eta} \cdot \bepsilon, \quad \bepsilon \sim \cN(0, \bI).
		\]
		will comes from $p(\bx | \btheta)$.
	\end{block}
	The density $p(\bx | \btheta)$ is a \textbf{stationary} distribution for the Langevin SDE.
	\myfootnotewithlink{https://www.stats.ox.ac.uk/~teh/research/compstats/WelTeh2011a.pdf}{Welling M. Bayesian Learning via Stochastic Gradient Langevin Dynamics, 2011}
\end{frame}
%=======
\begin{frame}{Outline}
	\tableofcontents
\end{frame}
%=======
\section{Probability flow ODE}
%=======
\begin{frame}{Probability flow ODE}
	\begin{block}{Theorem}
		Assume SDE $d\bx = \mathbf{f}(\bx, t) dt + g(t) d \bw$ induces the probability path $p(\bx, t)$.
		Then there exists ODE with identical probability path $p(\bx, t)$ of the form
		\vspace{-0.3cm}
		\[
			d\bx = \left[\mathbf{f}(\bx, t) -\frac{1}{2} g^2(t) \frac{\partial}{\partial \bx} \log p(\bx, t) \right] dt
		\]
		\vspace{-0.7cm}
	\end{block}
	\begin{block}{Proof}
 		\vspace{-0.7cm}
 		{\small
 		\begin{multline*}
 			\frac{\partial p(\bx, t)}{\partial t} = \text{tr}\left(- \frac{\partial}{\partial \bx} \bigl[ \mathbf{f}(\bx, t) p(\bx, t)\bigr] + \frac{1}{2} g^2(t) \frac{\partial^2 p(\bx, t)}{\partial \bx^2} \right) = \\
 			=  \text{tr}\left(- \frac{\partial}{\partial \bx} \left[ \mathbf{f}(\bx, t) p(\bx, t) - \frac{1}{2} g^2(t) {\color{violet}\frac{\partial p(\bx, t)}{\partial \bx}} \right]  \right) = \\
			 =  \text{tr}\left(- \frac{\partial}{\partial \bx} \left[ \mathbf{f}(\bx, t) p(\bx, t) - \frac{1}{2} g^2(t) {\color{violet}p(\bx, t) \frac{\partial \log p(\bx, t)}{\partial \bx}} \right]  \right)= \\
		  =  \text{tr}\left(- \frac{\partial}{\partial \bx} \left[ \left( {\color{teal}\mathbf{f}(\bx, t) - \frac{1}{2} g^2(t) \frac{\partial \log p(\bx, t)}{\partial \bx}}\right) p(\bx, t) \right]  \right)
 		\end{multline*}
 		}
 	\end{block}
	\myfootnotewithlink{https://arxiv.org/abs/2011.13456}{Song Y., et al. Score-Based Generative Modeling through Stochastic Differential Equations, 2020}
\end{frame}
%=======
\begin{frame}{Probability flow ODE}
	\begin{block}{Theorem}
		Assume SDE $d\bx = \mathbf{f}(\bx, t) dt + g(t) d \bw$ induces the distribution $p(\bx, t)$.
		Then there exists ODE with identical probabilities distribution $p(\bx, t)$ of the form
		\vspace{-0.3cm}
		\[
			d\bx = \left[\mathbf{f}(\bx, t) -\frac{1}{2} g^2(t) \frac{\partial}{\partial \bx} \log p(\bx, t) \right] dt
		\]
		\vspace{-0.7cm}
	\end{block}
	\begin{block}{Proof (continued)}
 		\vspace{-0.7cm}
 		\begin{multline*}
 			\frac{\partial p(\bx, t)}{\partial t} =  \text{tr}\left(- \frac{\partial}{\partial \bx} \left[ \left( {\color{teal}\mathbf{f}(\bx, t) - \frac{1}{2} g^2(t) \frac{\partial \log p(\bx, t)}{\partial \bx}}\right) p(\bx, t) \right]  \right) =\\
 			  =  \text{tr}\left(- \frac{\partial}{\partial \bx} \left[ {\color{teal}\tilde{\mathbf{f}}(\bx, t)} p(\bx, t) \right]  \right)
 		\end{multline*}
 	\end{block}
 	\vspace{-1.0cm}
 	\[
 		d \bx = \tilde{\bff}(\bx, t) dt + 0 \cdot d \bw = \left[\mathbf{f}(\bx, t) -\frac{1}{2} g^2(t) \frac{\partial}{\partial \bx} \log p(\bx, t) \right] dt
 	\]
	\myfootnotewithlink{https://arxiv.org/abs/2011.13456}{Song Y., et al. Score-Based Generative Modeling through Stochastic Differential Equations, 2020}
\end{frame}
%=======
\begin{frame}{Probability flow ODE}
	\vspace{-0.5cm}
	\begin{align*}
		d\bx &= \mathbf{f}(\bx, t) dt + g(t) d \bw - \text{SDE} \\
		d\bx &= \left[\mathbf{f}(\bx, t) -\frac{1}{2} g^2(t) \frac{\partial}{\partial \bx} \log p(\bx, t) \right] dt  - \text{probability flow ODE}
	\end{align*}
	\vspace{-0.3cm}
	\begin{itemize}
		\item The term $\bs(\bx, t) = \frac{\partial}{\partial \bx} \log p(\bx, t)$ is a score function for continuous time.
		\item ODE has more stable trajectories.
	\end{itemize}
	\begin{figure}
		\includegraphics[width=0.75\linewidth]{figs/probability_flow}
	\end{figure}
	\myfootnotewithlink{https://arxiv.org/abs/2011.13456}{Song Y., et al. Score-Based Generative Modeling through Stochastic Differential Equations, 2020}
\end{frame}
%=======
\section{Reverse SDE}
%=======
\begin{frame}{Reverse SDE}
	\vspace{-0.3cm}
	\[
		d\bx = \mathbf{f}(\bx, t) dt, \quad \bx(t + dt) = \bx(t) + \mathbf{f}(\bx, t) dt
	\]
	Here $dt$ could be $>0$ or $<0$. 
	\begin{block}{Reverse ODE}
		Let $\tau = 1 - t$ ($d\tau = -dt$).
		\vspace{-0.3cm}
		\[
			d\bx = - \bff(\bx, 1 - \tau) d \tau
		\]
	\end{block}
	\vspace{-0.5cm}
	\begin{itemize}
		\item How to revert SDE $d\bx = \mathbf{f}(\bx, t) dt + g(t) d \bw$? 
		\item Wiener process gives the randomness that we have to revert.
	\end{itemize}
	\vspace{-0.3cm}
	\begin{block}{Theorem}
		There exists the reverse SDE for the SDE $d\bx = \mathbf{f}(\bx, t) dt + g(t) d \bw$ that has the following form
		\vspace{-0.3cm}
		\[
			d\bx = \left(\mathbf{f}(\bx, t) {\color{violet}- g^2(t) \frac{\partial \log p(\bx, t)}{\partial \bx}}\right) dt + g(t) d \bw
		\]
		\vspace{-0.5cm} \\
		with $dt < 0$.
	\end{block}
	\myfootnotewithlink{https://arxiv.org/abs/2011.13456}{Song Y., et al. Score-Based Generative Modeling through Stochastic Differential Equations, 2020}
\end{frame}
%=======
\begin{frame}{Reverse SDE}
	\begin{block}{Theorem}
		There exists the reverse SDE for the SDE $d\bx = \mathbf{f}(\bx, t) dt + g(t) d \bw$ that has the following form
		\vspace{-0.3cm}
		\[
			d\bx = \left(\mathbf{f}(\bx, t) {\color{violet}- g^2(t) \frac{\partial \log p(\bx, t)}{\partial \bx}}\right) dt + g(t) d \bw
		\]
		\vspace{-0.5cm} \\
		with $dt < 0$.
	\end{block}
	\textbf{Note:} Here we also see the score function $\bs(\bx, t) = \frac{\partial}{\partial \bx} \log p(\bx, t)$.
	\begin{block}{Sketch of the proof}
		\begin{itemize}
			\item Convert initial SDE to probability flow ODE.
			\item Revert probability flow ODE.
			\item Convert reverse probability flow ODE to reverse SDE.
		\end{itemize}
	\end{block}
	\myfootnotewithlink{https://arxiv.org/abs/2011.13456}{Song Y., et al. Score-Based Generative Modeling through Stochastic Differential Equations, 2020}
\end{frame}
%=======
\begin{frame}{Reverse SDE}
	\begin{block}{Proof}
		\begin{itemize}
			\item Convert initial SDE to probability flow ODE
			\vspace{-0.1cm}
			{\footnotesize
			\begin{align*}
				d\bx &= \mathbf{f}(\bx, t) dt + g(t) d \bw \\
				d\bx &= \left[\mathbf{f}(\bx, t) -\frac{1}{2} g^2(t) \frac{\partial}{\partial \bx} \log p(\bx, t) \right] dt
			\end{align*}
			}
			\item Revert probability flow ODE
			\vspace{-0.1cm}
			{\footnotesize
			\begin{align*}
				d\bx &= \left[\mathbf{f}(\bx, t) -\frac{1}{2} g^2(t) \frac{\partial}{\partial \bx} \log p(\bx, t) \right] dt \\
				d\bx &= \left[- \mathbf{f}(\bx, 1 - \tau) + \frac{1}{2} g^2(1 - \tau) \frac{\partial}{\partial \bx} \log p(\bx, 1 - \tau) \right] d \tau
			\end{align*}
			}
			\item Convert reverse probability flow ODE to reverse SDE
			\vspace{-0.1cm}
			{\footnotesize
			\begin{align*}
				d\bx &= \left[- \mathbf{f}(\bx, 1 - \tau) + \frac{1}{2} g^2(1 - \tau) \frac{\partial}{\partial \bx} \log p(\bx, 1 - \tau) \right] d \tau \\
				d\bx &= \left[- \mathbf{f}(\bx, 1 - \tau) + g^2(1 - \tau) \frac{\partial}{\partial \bx} \log p(\bx, 1 - \tau) \right] d\tau + g(1 - \tau) d \bw
			\end{align*}
			}
		\end{itemize}
	\end{block}
	\myfootnotewithlink{https://arxiv.org/abs/2011.13456}{Song Y., et al. Score-Based Generative Modeling through Stochastic Differential Equations, 2020}
\end{frame}
%=======
\begin{frame}{Reverse SDE}
	\begin{block}{Theorem}
		There exists the reverse SDE for the SDE $d\bx = \mathbf{f}(\bx, t) dt + g(t) d \bw$ that has the following form
		\vspace{-0.3cm}
		\[
			d\bx = \left(\mathbf{f}(\bx, t) {\color{violet}- g^2(t) \frac{\partial \log p(\bx, t)}{\partial \bx}}\right) dt + g(t) d \bw
		\]
		\vspace{-0.5cm} \\
		with $dt < 0$.
	\end{block}
	\begin{block}{Proof (continued)}
		\vspace{-0.7cm}
		\[
			d\bx = \left[- \mathbf{f}(\bx, 1 - \tau) + g^2(1 - \tau) \frac{\partial}{\partial \bx} \log p(\bx, 1 - \tau) \right] d \tau + g(1 - \tau) d \bw
		\]
		\[
			d\bx = \left(\mathbf{f}(\bx, t) - g^2(t) \frac{\partial \log p(\bx, t)}{\partial \bx}\right) dt + g(t) d \bw
		\]
		Here $d\tau > 0$ and $dt < 0$.
	\end{block}
	\myfootnotewithlink{https://arxiv.org/abs/2011.13456}{Song Y., et al. Score-Based Generative Modeling through Stochastic Differential Equations, 2020}
\end{frame}
%=======
\begin{frame}{Reverse SDE}
	\vspace{-0.5cm}
	\begin{align*}
		d\bx &= \mathbf{f}(\bx, t) dt + g(t) d \bw - \text{SDE} \\
		d\bx &= \left[\mathbf{f}(\bx, t) -\frac{1}{2} g^2(t) \frac{\partial}{\partial \bx} \log p(\bx, t) \right] dt - \text{probability flow ODE} \\
		d\bx &= \left(\mathbf{f}(\bx, t) - g^2(t) \frac{\partial \log p(\bx, t)}{\partial \bx}\right) dt + g(t) d \bw - \text{reverse SDE}
	\end{align*}
	\vspace{-0.5cm}
	\begin{itemize}
		\item We got the way to transform one distribution to another via SDE with some probability path $p(\bx, t)$.
		\item We are able to revert this process with the score function.
	\end{itemize}
	\vspace{-0.3cm}
	\begin{figure}
		\includegraphics[width=0.9\linewidth]{figs/sde}
	\end{figure}
	\myfootnotewithlink{https://arxiv.org/abs/2011.13456}{Song Y., et al. Score-Based Generative Modeling through Stochastic Differential Equations, 2020}
\end{frame}
%=======
\section{Diffusion and Score matching SDEs}
%=======
\begin{frame}{Score matching SDE}
	\begin{block}{Denoising score matching}
		\vspace{-0.7cm}
		\begin{align*}
			\bx_t &= \bx + \sigma_t \cdot \bepsilon_t, \quad p(\bx, \sigma_t) = \cN(\bx, \sigma_t^2 \cdot \bI) \\
			\bx_{t-1} &= \bx + \sigma_{t-1} \cdot \bepsilon_{t-1}, \quad p(\bx, \sigma_{t-1}) = \cN(\bx, \sigma_{t-1}^2 \cdot \bI)
		\end{align*}
	\end{block}
	\vspace{-1.0cm}
	\[
		\bx_t = \bx_{t - 1} + \sqrt{\sigma^2_t - \sigma^2_{t-1}} \cdot \bepsilon, \quad q(\bx_{t} | \bx_{t-1}) = \cN(\bx_{t-1}, (\sigma_t^2 - \sigma_{t-1}^2) \cdot \bI)
	\]
	Let turn this Markov chain to the continuous stochastic process~$\bx(t)$ taking $T \rightarrow \infty$:
	\[
		{\color{teal}\bx(t + dt)} = {\color{teal}\bx(t)} + \sqrt{\frac{\sigma^2(t + dt) - \sigma^2(t)}{dt} {\color{violet}dt}} \cdot {\color{violet}\bepsilon} = \bx(t) + \sqrt{\frac{ d [\sigma^2(t)]}{dt}} \cdot {\color{violet}d \bw}
	\]
	\vspace{-0.5cm}
	\begin{block}{Variance Exploding SDE}
		\vspace{-0.3cm}
		\[
			d \bx = \sqrt{\frac{ d [\sigma^2(t)]}{dt}} \cdot d \bw
		\]
	\end{block}
	\myfootnotewithlink{https://arxiv.org/abs/2011.13456}{Song Y., et al. Score-Based Generative Modeling through Stochastic Differential Equations, 2020}
\end{frame}
%=======
\begin{frame}{Diffusion SDE}
	\begin{block}{Denoising Diffusion}
		\vspace{-0.5cm}
		\[
			\bx_t = \sqrt{1 - \beta_t} \cdot \bx_{t - 1} + \sqrt{\beta_t} \cdot \bepsilon, \quad q(\bx_t | \bx_{t-1}) = \cN(\sqrt{1 - \beta_t} \cdot \bx_{t-1}, \beta_t \cdot \bI)
		\]
		\vspace{-0.5cm}
	\end{block}
	Let turn this Markov chain to the continuous stochastic process taking $T \rightarrow \infty$ and taking $\beta(\frac{t}{T}) = \beta_t \cdot T$
	\begin{multline*}
		{\color{teal}\bx(t)} = \sqrt{1 - \beta(t) dt} \cdot \bx(t - dt) + \sqrt{\beta(t)dt} \cdot \bepsilon \approx \\
		\approx (1 - \frac{1}{2} \beta(t) dt) \cdot \bx(t - dt) + \sqrt{\beta(t){\color{violet}dt}} \cdot {\color{violet}\bepsilon} = \\
		= {\color{teal}\bx(t - dt)} - \frac{1}{2} \beta(t) \bx(t - dt) dt  + \sqrt{\beta(t)} \cdot {\color{violet}d \bw}
	\end{multline*}
	\vspace{-0.5cm}
	\begin{block}{Variance Preserving SDE}
		\vspace{-0.3cm}
		\[
			{\color{teal}d \bx} = - \frac{1}{2} \beta(t) \bx(t) dt + \sqrt{\beta(t)} \cdot d \bw
		\]
	\end{block}
	\myfootnotewithlink{https://arxiv.org/abs/2011.13456}{Song Y., et al. Score-Based Generative Modeling through Stochastic Differential Equations, 2020}
\end{frame}
%=======
\begin{frame}{Diffusion SDE}
	\vspace{-0.3cm}
	\[
		d\bx = \mathbf{f}(\bx, t) dt + g(t) d \bw
	\]
	\vspace{-0.3cm}
	\begin{block}{Variance Exploding SDE (NCSN)}
		\vspace{-0.5cm}
		\[
			d \bx = \sqrt{\frac{ d [\sigma^2(t)]}{dt}} \cdot d \bw, \quad \bff(\bx, t) = 0, \quad g(t) = \sqrt{\frac{ d [\sigma^2(t)]}{dt}} 
		\]
		Variance grows since $\sigma(t)$ is a monotonically increasing function.
	\end{block}
	\begin{block}{Variance Preserving SDE (DDPM)}
		\vspace{-0.3cm}
		\[
			d \bx = - \frac{1}{2} \beta(t) \bx(t) dt + \sqrt{\beta(t)} \cdot d \bw
		\]
		\[
			\bff(\bx, t) = - \frac{1}{2} \beta(t) \bx(t) , \quad g(t) = \sqrt{\beta(t)} 
		\]
		Variance is preserved if $\bx(0)$ has a unit variance.
	\end{block}
	\myfootnotewithlink{https://arxiv.org/abs/2011.13456}{Song Y., et al. Score-Based Generative Modeling through Stochastic Differential Equations, 2020}
\end{frame}
%=======
\begin{frame}{Summary}
	\begin{itemize}
		\item There exists special probability flow ODE for each SDE that gives the same probability path.
		\vfill
		\item It is possible to revert SDE using score function.
		\vfill
		\item Score matching (NCSN) and diffusion models (DDPM) are the discretizations of the SDEs (variance exploding and variance preserving).
	\end{itemize}
\end{frame}
\end{document} 